Leo
In english, 

### Exercise Sheet 1 (Week 37-1)
1. First
	1. F
	2. T
	3.  F
	4. T


### Exercise Sheet 2 (Week 37-2)
1.  
    a.  

## Exercise Sheet 6 (Week 39-2)
1.
$$
\begin{align}
\frac{1}{1\cdot2} &=\frac{1}{2} \\
\frac{1}{2\cdot 3}+\frac{1}{1\cdot2} &=\frac{4}{6} \\
\frac{1}{3\cdot4}+\frac{1}{2\cdot 3}+\frac{1}{1\cdot2} &=\frac{9}{12} \\
 \\
\sum_{i=1}^{n} \frac{1}{i(i+1)}&=\frac{n^{2}}{n(n+1)}
\end{align}
$$


$$
\begin{align}
&=\sum_{i=1}^{k} \frac{1}{i(i+1)}+\frac{1}{(k+1)(k+1+1)} \\
&=\frac{k^{2}}{k(k+1)}+ \frac{1}{(k+1)(k+2)} \text{ hyptese brugt} \\
&=\frac{(k+2)\cdot k^{2}}{k(k+2)(k+1)}+\frac{k}{k(k+1)(k+2)} \\
&=\frac{(k+2)\cdot k^{2}+k}{k(k+2)(k+1)} \\
&=\frac{k^{2}+2k+1}{(k+2)(k+1)} \\
&=\frac{(k+1)^{2}}{(k+2)(k+1)} \\
\end{align}
$$

2.  exersice 2
	1. $\{x \in \mathbb{N}\mid x < 13 \text{ is multiplu of 3}\} = \{x \in \mathbb{N}\mid \exists k \in \mathbb{N}:(x=3k \vee k\leq 4 )\}$
	2. $\{x \in \mathbb{Z} \mid |x|\leq 3 \}$
	 exersie 11
	  yes
	  no
	  no
17
3. Y
4. Y
5. no
6. Y
7. Y
8. N
25
9. 1
10. 1
11. 2
12. 3
27
a. $\{\emptyset, \{a\}\}$
b. $\{\emptyset, \{a\},\{b\},\{a,b\}\}$
c. $\{\emptyset, \{\emptyset\},\{\{\emptyset\}\},\{\emptyset,\{\emptyset\}\}\}$


## Exercise Sheet 7 (Week 40)
1. section 2.2
	- e.21
2. $S_{4},S_{5},S_{6},S_{7}$
3. section 2.1
	* e33
		* $\{a,b,c,d\}\times \{y,z\}=\{(a,y),(a,z),(b,y),(b,z),(c,y),(c,z),(d,y),(d,z),\}$
		* $\{y,z\}\times\{a,b,c,d\}=\{(y,a),(y,b),(y,c),(y,d),(z,a),(z,b),(z,c),(z,d)\}$
4. section 2.2 
	- e31g
		- a) $B \subseteq A$
		- b) $A \subseteq B$
		- c) $A\cap B=\emptyset$
		- d) is comemntive
		- E) $A=B$
5. section 2.3
	- e1:
		- not define for $x=0$
		- not define for $x<0$
		- tvetydig, en værdi kan give $\pm$
##  Exercise Sheet 8 (Week 41-1)
1. section 2.3
12.

T,  F, T, F
13.
T, F, F, T
(a is bijective)
38.
$f\circ g=(x+2)^{2}+1=x^{2}+4x+5$
$g\circ f=x^{2}+1+2=x^{2}+3$
39.
$(f+g)(x)=x^{2}+1+x+2=x^{2}+x+3$
$(f\cdot g)(x)=(x^{2}+1)(x+2)=x^{3}+2x^{2}+x+2$

71.
$f^{-1}(y)=\sqrt[3]{y-1}$


2.
* is true,
* is false
* is false
* is true


1. section 2.5
2.
$\aleph_{0}$    $\mathbb{Z}^{+}+10$
, finite,
$\aleph_{0}$


# Exercise Sheet 9 (Week 41-2)
1. section 2.5
exsoerise2
b)$\aleph_{0}$ ($f(x)=-2x+1, x \in \mathbb{Z}^+$)d) uncoutable inftinete f) $\aleph_{0}, \ \ f(x)=10, x \in \mathbb{Z}^+$
exersise 10 
a. $A=\mathbb{N}, B=\mathbb{Z}^+$, $A=[1,2], B=]1,2]$
b. $A=\mathbb{Z}, B=\mathbb{Z}^+$,     $A=[1,2]\cup \mathbb{Z}, B=[1,2]$     $\mathbb{R}-\mathbb{R}|\mathbb{Q}=\mathbb{Q}$
c. $A=\mathbb{R}, B=\mathbb{R}^+$
exersice 17
yes

2. section 5.3
ecserice 1
a.
$$
\begin{align}
f(0) & =1 \\
f(n+1) & = f(n)+2 \\ \\
f(1) & =3 \\
f(2) & =5 \\
f(3) & =7 \\
f(4) & =9
\end{align}
$$
b.
$$
\begin{align}
f(0) & =1 \\
f(n+1) & = 3f(n) \\ \\
f(1) & =3 \cdot 1 & =3 \\
f(2) & =3\cdot 3 & =9 \\
f(3) & =3 \cdot 9 & =27 \\
f(4) & =3\cdot 27 & =81
\end{align}
$$
exsicce 7
a.
$a(1)=6, a(n+1)=a(n)+6, n>1$
b.
$a(0)=1, a(n+1)=a(n)+2, n\geq 0$

3.
Prove that for all n ∈ N with n ≥ 8, there exist a, b ∈ N with n = 3a + 5b.
$$
\begin{align}  
P(n)=3a+5b,  & \ a,b\in \mathbb{N}\\
\text{Basecase: } 8, 9 ,10 \\  
P(8) & =3\cdot 1+5\cdot 1  & = 8\\
P(9) & =3\cdot 3+5\cdot 0  & = 9\\
P(10) & =3\cdot 0+5\cdot 10 & = 10 \\
 \\ 
\text{inductions antagle} \\
 P(k-3)  & \implies P(k), k\geq 11\\
 k-3 & =3\cdot a + 5 \cdot b &\ a,b\in \mathbb{N}\\ \\
\text{induktiions skridt} \\
k & =(k-3)+3 \\
k & = 3\cdot a + 5 \cdot b +3, &  \ a,b \in \mathbb{N}& \text{ ved ind. hyp} \\ 
k & = 3\cdot a + 3+ 5 \cdot b , &  \ a,b \in \mathbb{N} \\
k  & = 3(a + 1)+ 5 \cdot b , &  \ (a+1),b \in \mathbb{N} \\
 &  &  &  \square
\end{align}
$$Does there exist a number k ∈ N such that, for all n ∈ N with n ≥ k, there
exist a, b ∈ N with n = 4a + 5b?
$k=12$



$1\in Odd \wedge 1\in \mathbb{N}$

2. section 5.3
excisece 27
a) odd postive integes
b)  $\mathbb{Z}^+$
c) $\{n\in \mathbb{Z}|k \in \mathbb{N},n=2^k\}$
d) $\mathbb{Z}^+$

excise 12
$$
\begin{align}  \\
n\implies n-1 \\
P(n)=n-1 \\
 \\

\text{Basis step}  \\

P(1) & = 1-1=0\\ \\

\text{induktunios hyptose step} \\
[P(1)\wedge P(2)\wedge \dots \wedge P(k)] & \implies P(k+1) \\ 
[P(1)\wedge P(2)\wedge \dots \wedge P(k)] & \implies k+1-1 \\ 
 \\
\text{induktions skridt} \\
k+1 & = P(a) + P(b),  & a+b &=(k+1)
\end{align}
$$